theories/opt/ex2_down.v
@@ -2,26 +2,28 @@ From stbor.sim Require Import local invariant refl_step.
 
 Set Default Proof Using "Type".
 
+(** Moving a read of a shared reference down across code that *may* use that ref. *)
+
 (* Assuming x : & i32 *)
-Definition ex2_2 : function :=
+Definition ex2_down : function :=
   fun: ["i"],
-    let: "x" := new_place (& int) &"i" in
+    let: "x" := new_place (& int) "i" in
     Retag "x"  FnEntry ;;
     let: "v" := Copy *{int} "x" in
     Call #[ScFnPtr "f"] ["x"] ;;
     "v"
     .
 
-Definition ex2_2_opt : function :=
+Definition ex2_down_opt : function :=
   fun: ["i"],
-    let: "x" := new_place (& int) &"i" in
+    let: "x" := new_place (& int) "i" in
     Retag "x"  FnEntry ;;
     Call #[ScFnPtr "f"] ["x"] ;;
     Copy *{int} "x"
     .
 
 
-Lemma ex2_2_sim_fun fs ft : ⊨{fs,ft} ex2_2 ≥ᶠ ex2_2_opt.
+Lemma ex2_down_sim_fun fs ft : ⊨{fs,ft} ex2_down ≥ᶠ ex2_down_opt.
 Proof.
   intros r es et els elt σs σt FAs FAt FREL SUBSTs SUBSTt.
   destruct els as [|efs []]; [done| |done].  simpl in SUBSTs.
