theories/opt/ex2.v
@@ -2,10 +2,12 @@ From stbor.sim Require Import local invariant refl_step.
 
 Set Default Proof Using "Type".
 
+(** Moving read of shared ref up across code that *may* use that ref. *)
+
 (* Assuming x : & i32 *)
 Definition ex2 : function :=
   fun: ["i"],
-    let: "x" := new_place (& int) &"i" in
+    let: "x" := new_place (& int) "i" in
     Retag "x" Default ;;
     Copy *{int} "x" ;;
     Call #[ScFnPtr "f"] ["x"] ;;
@@ -14,7 +16,7 @@ Definition ex2 : function :=
 
 Definition ex2_opt : function :=
   fun: ["i"],
-    let: "x" := new_place (& int) &"i" in
+    let: "x" := new_place (& int) "i" in
     Retag "x" Default ;;
     Copy *{int} "x" ;;
     let: "v" := Copy *{int} "x" in
