theories/opt/ex3_down.v
@@ -1,0 +1,46 @@
+From stbor.sim Require Import local invariant refl_step.
+
+Set Default Proof Using "Type".
+
+(** Moving a write to a mutable reference down across unknown code. *)
+
+(* Assuming x : &mut i32 *)
+Definition ex3_down : function :=
+  fun: ["i"],
+    let: "x" := new_place (&mut int) "i" in
+    Retag "x"  FnEntry ;;
+    *{int} "x" <- #[42] ;;
+    let: "v" := Call #[ScFnPtr "f"] [] in
+    *{int} "x" <- #[13] ;;
+    "v"
+  .
+
+Definition ex3_down_opt_1 : function :=
+  fun: ["i"],
+    let: "x" := new_place (&mut int) "i" in
+    Retag "x"  FnEntry ;;
+    let: "v" := Call #[ScFnPtr "f"] [] in
+    *{int} "x" <- #[42] ;;
+    *{int} "x" <- #[13] ;;
+    "v"
+  .
+
+Definition ex3_down_opt_2 : function :=
+  fun: ["i"],
+    let: "x" := new_place (&mut int) "i" in
+    Retag "x"  FnEntry ;;
+    let: "v" := Call #[ScFnPtr "f"] [] in
+    *{int} "x" <- #[13] ;;
+    "v"
+  .
+
+Lemma ex3_down_sim_fun fs ft : ⊨{fs,ft} ex3_down ≥ᶠ ex3_down_opt_1.
+Proof.
+  intros r es et els elt σs σt FAs FAt FREL SUBSTs SUBSTt.
+  destruct els as [|efs []]; [done| |done].  simpl in SUBSTs.
+  destruct elt as [|eft []]; [done| |done].  simpl in SUBSTt. simplify_eq.
+
+  (* InitCall *)
+  exists 10%nat.
+  apply sim_body_init_call. simpl.
+Abort.
